Deploying to gh-pages from @ xubaiw/reservoir-index@3617a3048f6e3e4e27beee1ea788a3ed80405121 🚀

git/rebryant/model-counting/crat/prototype/crat_checker.py
@@ -955,7 +955,7 @@ class Prover:
         root = self.cmgr.root
         if root is None:
             print("Can't determine count.  Don't know root")
-            return 0.0
+            return P52()
         return self.omgr.count(self.cmgr.root, weights)
 
     def invalidCommand(self, cmd):
