git/rebryant/model-counting/crat/prototype/pigeon-dsharp/prun.sh
@@ -1,0 +1,7 @@
+#!/bin/bash
+for N in {3..8}
+do
+    make psd-all N=$N
+    make pst-all N=$N
+done
+
